WIP: escrowAgent transfer verifies with PromiseT<T> = T

packages/zoe/spec/escrowAgent.dfy
@@ -1,63 +1,107 @@
 include "amountMath.dfy"
 include "elib.dfy"
+include "outcome.dfy"
+
+module Far {
+  function E<T>(rx: T): T { rx }
+}
 
 abstract module ERTP {
   import ELib
+  import A = M0.AmountMath
+  import O = Outcome
 
   trait Brand extends ELib.Callable {
-    function isMyIssuer(i: Issuer): bool
+    function isMyIssuer(i: Issuer): bool reads this
   }
   trait Issuer extends ELib.Callable {
-    function getBrand(): Brand
+    function getBrand(): Brand reads this
     method makeEmptyPurse() returns (p: Purse)
+        modifies this.reach
+        ensures p.reach == this.reach + { p }
   }
 
   trait Purse extends ELib.Callable {
-    function getAllegedBrand(): Brand
+    function getAllegedBrand(): Brand reads this
+    method deposit(amount: A.Amount, srcPurse: Purse) returns (ret: O.Outcome<A.Amount>)
+        // modifies this.reach, srcPurse.reach
+  }
+}
+
+module AsyncJS {
+  import O = Outcome
+  type PromiseT<T> = T
+  function awaitO<T>(po: O.Outcome<T>): O.Outcome<T> { po }
+  function await<T>(p: PromiseT<T>): O.Outcome<T> { O.Success(p) }
+  class Promise {
+    static function all<T, U>(ps: (PromiseT<T>, PromiseT<U>)): O.Outcome<(T, U)> { O.Success(ps) }
+    static function race<T>(ps: seq<PromiseT<T>>): O.Outcome<T> {
+      if |ps| > 0 then O.Success(ps[0]) else O.Failure("empty race")
+    }
+
+  }
+}
+
+module Q {
+  import O = Outcome
+  import opened AsyncJS
+
+  method join<T(==)>(a: PromiseT<T>, b: PromiseT<T>) returns (ret: O.Outcome<T>) {
+    var abr: (T, T) :- awaitO(Promise.all((a, b)));
+    var ar, br := abr.0, abr.1;
+    if (ar != br) {
+      return O.Failure("join failed");
+    }
+    return O.Success(ar);
   }
 }
 
 abstract module Escrow {
   import opened M0.AmountMath
   import opened ERTP
-  import opened ELib
+  import ELib
   import opened Passable
+  import opened Far
+  import opened AsyncJS
+  import O = Outcome
+  import Q
 
-  class EscrowVat extends E {
+  type Result<T> = O.Outcome<T>
+
+  class EscrowVat extends ELib.E {
     var issuer0: Issuer // TODO set/seq of issuers
 
     constructor(i0: Issuer) {
-      var reason := new Fail("BROKEN");
-      theBroken := new UnconnectedRef(reason);
+      var reason := new ELib.Fail("BROKEN");
+      theBroken := new ELib.UnconnectedRef(reason);
       issuer0 := i0;
     }
 
-    method transfer(decisionP: Ref, srcPurseP: Ref, dstPurse: Ref, amount: Amount) returns (ret: Ref) // Promise<Amount>
+    method transfer(decisionP: O.Outcome<()>, srcPurseP: PromiseT<Purse>, dstPurseP: PromiseT<Purse>, amount: Amount)
+      returns (ret: O.Outcome<Amount>)
       requires srcPurseP.CapOK()
-      modifies srcPurseP.reach
+      modifies srcPurseP.reach, dstPurseP.reach
+      modifies issuer0.reach
     {
-      // var q := decisionP.Home();
-      // var makeEscrowPurseP := q.join(
-      //   E.get(srcPurseP).makePurse,
-      //   E.get(dstPurseP).makePurse
-      // );
-      var srcBrandP := this.sendAll(srcPurseP, "getAllegedBrand", []);
-      var x := srcBrandP.MoveNext(); // a la await
+      var srcBrandP := Q.join(E(srcPurseP).getAllegedBrand(), E(dstPurseP).getAllegedBrand());
+      var srcBrand :- awaitO(srcBrandP);
+      if (srcBrand != issuer0.getBrand()) {
+        return O.Failure("brand / issuer mismatch");
+      }
+      var escrowPurseP := E(issuer0).makeEmptyPurse();
 
-      var srcBrand :- srcBrandP.MoveNext(); // a la await
-      //   if (srcBrand != Value.Remotable(issuer0.getBrand())) {
-      //     return broken(); // reason: brand / issuer mismatch
-      //   }
-      // // setup phase 2
-      // var yes := new DepositIt(dstPurseP, amount, escrowPurseP);
-      // var no := new DepositIt(srcPurseP, amount, escrowPurseP);
-      // decisionP.Then( // defensive: q.promise(decisionP).then...
-      //   yes
-      // ).Catch(no);
+      // OK to do phase 1 before phase 2?
+      ret := E(escrowPurseP).deposit(amount, srcPurseP); // phase 1
 
-      // ret := E(escrowPurseP).deposit(amount, srcPurseP); // phase 1
-      ret := broken(); // TODO
+      // setup phase 2
+      match await(decisionP) {
+        case Success(_) => {
+          var ignore := E(dstPurseP).deposit(amount, escrowPurseP);
+        }
+        case Failure(_) => {
+          var ignore := E(srcPurseP).deposit(amount, escrowPurseP);
+        }
+      }
     }
-
   }
 }
